coq/SigmaHCOL/SigmaHCOLMem.v
@@ -1068,6 +1068,26 @@ Section Operators.
        | List.cons b l => f (fold_left_rev f a l) b
        end.
 
+  Global Instance fold_left_rev_proper
+         {A B : Type}
+         `{Eb: Equiv B}
+         `{Ae: Equiv A}
+         `{Equivalence A Ae}
+         (f : A -> B -> A)
+         `{f_mor: !Proper ((=) ==> (=) ==> (=)) f}
+         (a : A)
+    :
+      Proper ((=) ==> (=)) (fold_left_rev f a).
+  Proof.
+    intros x y E.
+    induction E.
+    -
+      reflexivity.
+    -
+      simpl.
+      apply f_mor; auto.
+  Qed.
+
   Program Fixpoint Lbuild {A: Type}
           (n : nat)
           (gen : forall i, i < n -> A) {struct n}: list A :=
